Checkpoint

src/tls/HMAC.UFCMA.fst
@@ -5,38 +5,45 @@ open Mem
 open Platform.Bytes
 open Platform.Error
 
-module MM = FStar.Monotonic.Map 
+module MM = FStar.Monotonic.Map
 
 // idealizing HMAC
 // for concreteness; the rest of the module is parametric in a:alg
 
 // To be moved to Flags.
-assume val ideal: bool
+let model = Flags.model
+assume val ideal: b:bool{b ==> model}
+let ipkg = IK.ipkg
+type safe (#ip:ipkg) (i:ip.IK.t) = ideal /\ ip.IK.honest i
 
- 
-//let _ = assert false 
+let is_safe (#ip:ipkg) (i:ip.IK.t{ip.IK.registered i})
+  : ST bool (requires fun h0 -> True)
+  (ensures fun h0 b h1 -> modifies_none h0 h1 /\ (b <==> safe i))
+  =
+  let b = ip.IK.get_honesty i in
+  ideal && b
+
+//let _ = assert false
 
 #set-options "--initial_fuel 1 --max_fuel 1 --initial_ifuel 1 --max_ifuel 1"
 
-type ha = Hashing.Spec.alg 
+type ha = Hashing.Spec.alg
 type text = bytes
 
-noeq type info: Type0 = { 
+noeq type info: Type0 = {
   parent: r:rgn {~ (is_tls_rgn r)};
-  alg: Hashing.Spec.alg; //too loose? IK.kdfa; 
+  alg: Hashing.Spec.alg; //too loose? IK.kdfa;
   good: text -> bool (*TODO: should be Type0 *)}
 
 type tag (u:info) = lbytes (Hashing.Spec.tagLen u.alg)
 
 let keylen (u:info): IK.keylen = UInt32.uint_to_t (Hashing.Spec.tagLen u.alg)
-type keyrepr (u:info) = Hashing.Spec.hkey u.alg 
+type keyrepr (u:info) = Hashing.Spec.hkey u.alg
 
-let ipkg = IK.ipkg  
-
-let goodish (#ip:ipkg) (i:ip.IK.t) (u:info) (msg:text) = 
+let goodish (#ip:ipkg) (i:ip.IK.t) (u:info) (msg:text) =
   _: unit{
-  (~ ideal)\/ 
-  ip.IK.corrupt i \/ 
+  (~ ideal)\/
+  ip.IK.corrupt i \/
   u.good msg}
 
 private type log_t
@@ -46,44 +53,66 @@ private type log_t
   (r:rgn)
 = MM.t r (tag u * text) (fun (t,v) -> goodish i u v) (fun _ -> True) // could constrain size
 
-// readers and writers share the same private state: a log of MACed messages
-noeq abstract type key (ip:ipkg) (i:ip.IK.t) =
-  | Key:
-    u: info -> // creation-time parameters, kept for convenience
-    region: Mem.subrgn u.parent {~(is_tls_rgn region)} ->  // intuitively, the writer's region
-    kv: keyrepr u ->
-    log: log_t i u region -> //TODO: make conditional
-    key ip i 
+// The runtime (concrete) type of MAC instances
+noeq abstract type concrete_key =
+  | MAC: u:info -> k:keyrepr u -> concrete_key
 
-val region: #ip:ipkg -> #i:ip.IK.t -> k:key ip i -> GTot (subrgn k.u.parent)
-val keyval: #ip:ipkg -> #i:ip.IK.t -> k:key ip i -> GTot (keyrepr k.u)
+// The model type of instances - either ideal, or real
+noeq abstract type ir_key (ip:ipkg) (i:ip.IK.t) =
+  | IdealKey:
+    ck: concrete_key ->
+    region: Mem.subrgn ck.u.parent {~(is_tls_rgn region)} ->  // intuitively, the writer's region
+    log: log_t i ck.u region ->
+    ir_key ip i
+  | RealKey: ck:concrete_key -> ir_key ip i
 
-let region #ip #i k  = k.region
-let keyval #ip #i k = k.kv
+type key (ip:ipkg) (i:ip.IK.t) =
+  (if model then
+    k:ir_key ip i{IdealKey? k <==> safe i}
+  else concrete_key)
 
-private let gen (ip:ipkg) (i:ip.IK.t) (u:info) (kv:keyrepr u) : ST (k:key ip i)
-  (requires (fun _ -> True))
-  (ensures (fun h0 k h1 ->
-    k.u == u /\
-    fresh_subregion (region k) u.parent h0 h1 /\
-    modifies Set.empty h0 h1
-  )) =
+let usage (#ip:ipkg) (#i:ip.IK.t) (k:key ip i) : GTot info =
+  if model then
+    match k <: ir_key ip i with
+    | IdealKey ck _ _ -> ck.u
+    | RealKey ck -> ck.u
+  else k.u
+
+let keyval (#ip:ipkg) (#i:ip.IK.t) (k:key ip i) : GTot (keyrepr (usage k)) =
+  if model then
+    match k <: ir_key ip i with
+    | IdealKey ck _ _ -> ck.k
+    | RealKey ck -> ck.k
+  else k.k
+
+let region (#ip:ipkg) (#i:ip.IK.t) (k:key ip i)
+  : Ghost (subrgn (usage k).parent)
+  (requires safe i) (ensures fun _ -> True)
+  = let IdealKey _ r _ = k <: ir_key ip i in r
+
+let footprint (#ip:ipkg) (#i:ip.IK.t {ip.IK.registered i}) (k:key ip i) : IK.rset =
+  if model then
+    match k <: ir_key ip i with
+    | IdealKey _ r _ -> assume false; Set.singleton r // FIXME downwards closed set
+    | RealKey _ -> Set.empty
+  else Set.empty
+
+val create:
+  ip:ipkg -> ha_of_i: (ip.IK.t -> ha) -> good_of_i: (ip.IK.t -> text -> bool) ->
+  i:ip.IK.t {ip.IK.registered i} ->
+  u:info {u.alg = ha_of_i i /\ u.good == good_of_i i} -> ST (k:key ip i)
+  (requires fun _ -> model)
+  (ensures fun h0 k h1 ->
+    modifies Set.empty h0 h1 /\
+    usage k == u /\
+    IK.fresh_regions (footprint k) h0 h1)
+
+let create ip _ _ i u =
   let region: Mem.subrgn u.parent = new_region u.parent in
   assert(~(is_tls_rgn u.parent));
-  let log: log_t #ip i u region = MM.alloc #_ #_ #_ #_ in 
-  Key u region kv log
-
-val create: 
-  ip:ipkg -> ha_of_i: (ip.IK.t -> ha) -> good_of_i: (ip.IK.t -> text -> bool) ->
-  i:ip.IK.t {ip.IK.registered i} -> 
-  u:info {u.alg = ha_of_i i /\ u.good == good_of_i i} -> ST (k:key ip i)
-  (requires (fun _ -> True))
-  (ensures (fun h0 k h1 ->
-    modifies Set.empty h0 h1 /\
-    k.u == u /\
-    Mem.fresh_subregion (region k) u.parent h0 h1 ))
-let create ip _ _ i u =
+  let log: log_t #ip i u region = MM.alloc #_ #_ #_ #_ in
   let kv: keyrepr u = CoreCrypto.random (Hashing.Spec.tagLen u.alg) in
+<<<<<<< HEAD
   gen ip i u kv 
 
 // placeholder; will require allocating the sub-region only ideally.
@@ -95,11 +124,32 @@ assume val coerceT:
   key ip i
 
 val coerce: 
+=======
+  let ck = MAC u kv in
+  let k : ir_key ip i =
+    if is_safe i then
+      IdealKey ck region log
+    else
+      RealKey ck in
+  k <: key ip i
+
+let coerceT (ip: ipkg) (ha_of_i: ip.IK.t -> ha) (good_of_i: ip.IK.t -> text -> bool)
+  (i: ip.IK.t {ip.IK.registered i}) (u: u:info {u.alg = ha_of_i i /\ u.good == good_of_i i})
+  (kv: IK.lbytes (keylen u))
+  : Ghost (key ip i) (requires ~(safe i)) (ensures fun _ -> True) =
+  let ck = MAC u kv in
+  if model then
+    let k : ir_key ip i = RealKey ck in k
+  else ck
+
+val coerce:
+>>>>>>> Checkpoint
   ip: ipkg -> ha_of_i: (ip.IK.t -> ha) -> good_of_i: (ip.IK.t -> text -> bool) ->
-  i: ip.IK.t {ip.IK.registered i} -> 
+  i: ip.IK.t {ip.IK.registered i} ->
   u: (u: info {u.alg = ha_of_i i /\ u.good == good_of_i i}) ->
-  kv: IK.lbytes (keylen u) -> 
+  kv: IK.lbytes (keylen u) ->
   ST (k:key ip i)
+<<<<<<< HEAD
   (requires (fun _ -> ideal ==> ip.IK.corrupt i))
   (ensures (fun h0 k h1 ->
     modifies Set.empty h0 h1 /\
@@ -111,147 +161,158 @@ let coerce ip ha_of_i good_of_i i u kv =
   assume (k == coerceT ip ha_of_i good_of_i i u kv);
   k
 
+=======
+  (requires fun _ -> ~(safe i))
+  (ensures fun h0 k h1 ->
+    modifies_none h0 h1 /\
+    ~(safe i) /\ // annoying
+    k == coerceT ip ha_of_i good_of_i i u kv /\
+    usage k == u /\
+    IK.fresh_regions (footprint k) h0 h1)
+
+let coerce ip _ _ i u kv =
+  let ck = MAC u kv in
+  if model then
+    let k : ir_key ip i = RealKey ck in k
+  else ck
+>>>>>>> Checkpoint
 
 // not quite doable without reification?
 // assert_norm(forall ip i u. (create #ip i u == coerce #ip i u (CoreCrypto.random (UInt32.v (keylen u)))))
 
-val footprint:
-  ip: ipkg -> ha_of_i: (ip.IK.t -> ha) -> good_of_i: (ip.IK.t -> text -> bool) ->
-  #i: ip.IK.t {ip.IK.registered i} -> 
-  k: key ip i -> rset 
-let footprint _ _ _ #_ k = 
-  Set.singleton k.region
-
-unfold let info1 
-  (ip:ipkg) 
+unfold let info1
+  (ip:ipkg)
   (ha_of_i: ip.IK.t -> ha)
   (good_of_i: ip.IK.t -> text -> bool)
-  (i: ip.IK.t): Type0 
-= 
-  a:info{a.alg = ha_of_i i /\ a.good == good_of_i i} 
+  (i: ip.IK.t): Type0
+  =
+  a:info{a.alg = ha_of_i i /\ a.good == good_of_i i}
 
-unfold let localpkg 
-  (ip: ipkg) 
+unfold let localpkg
+  (ip: ipkg)
   (ha_of_i: i:ip.IK.t -> ha)
+<<<<<<< HEAD
   (good_of_i: ip.IK.t -> text -> bool) 
   : 
   p: IK.local_pkg ip {IK.LocalPkg?.info #ip p == info1 ip ha_of_i good_of_i}
 = 
+=======
+  (good_of_i: ip.IK.t -> text -> bool)
+  : p: IK.local_pkg ip {IK.LocalPkg?.info #ip p == info1 ip ha_of_i good_of_i}
+  =
+>>>>>>> Checkpoint
     IK.LocalPkg
       (fun (i:ip.IK.t {ip.IK.registered i}) -> key ip i)
       (info1 ip ha_of_i good_of_i)
-      (fun #_ u -> keylen u ) 
-      ideal  
-      // local footprint 
-      (fun #i (k:key ip i) -> Set.empty (*17-11-24 Set.singleton k.region *)  )
-      // local invariant 
-      (fun #_ k h -> True)
-      (fun r i h0 k h1 -> ())
-      // create/coerce postcondition
-      (fun #i u k h1 -> k.u == u (*17-11-24  /\ fresh_subregion (region k) u.parent h0 h1 *) )
+      (fun #_ u -> keylen u )
+      ideal
+      footprint // local footprint
+      (fun #_ k h -> True) // local invariant
+      (fun r i h0 k h1 -> ()) // Local invariant framing
+      (fun #i u k h1 -> usage k == u) // create/coerce postcondition
       (fun #i u k h1 r h2 -> ())
       (create ip ha_of_i good_of_i)
       (coerceT ip ha_of_i good_of_i)
       (coerce ip ha_of_i good_of_i)
 
-unfold 
-let pkg 
-  (ip:ipkg) 
+unfold
+let pkg
+  (ip:ipkg)
   (ha_of_i: ip.IK.t -> ha)
   (good_of_i: ip.IK.t -> text -> bool)
   (table: IK.mem_table (key ip))
   : IK.pkg ip
 //  (requires fun h0 -> True)
 //  (ensures fun h0 r h1 -> modifies_one tls_define_region h0 h1)
-= 
-  let p = localpkg ip ha_of_i good_of_i in 
+=
+  let p = localpkg ip ha_of_i good_of_i in
   //assert(p.IK.key == key ip);
   assert(IK.LocalPkg?.info #ip p == info1 ip ha_of_i good_of_i);
 
-  let table: IK.mem_table p.IK.key = admit() in //table in 
-  let q = IK.memoization p table in 
+  let table: IK.mem_table p.IK.key = admit() in //table in
+  let q = IK.memoization p table in
   assert(IK.Pkg?.key q == key ip);
   q
 
-val leak: 
-  #ip: ipkg -> 
-  #i: ip.IK.t -> 
+val leak:
+  #ip: ipkg ->
+  #i: ip.IK.t ->
   k: key ip i {ip.IK.corrupt i} -> kv:keyrepr k.u { kv = keyval k }
 let leak #_ #_ k = k.kv
 
-val mac: 
+val mac:
   #ip:ipkg -> #i:ip.IK.t -> k:key ip i ->
   p:text {ip.IK.corrupt i \/ k.u.good p} -> ST (tag k.u)
   (requires (fun _ -> True))
   (ensures (fun h0 t h1 -> modifies (Set.singleton (region k)) h0 h1 ))
-  // we may be more precise to prove ideal functional correctness, 
+  // we may be more precise to prove ideal functional correctness,
   // e,g,  /\ sel h1 k.log = snoc (sel h0 k.log) (Entry t p)
 let mac #ip #i k p =
-  let kv: keyrepr k.u = k.kv in  
+  let kv: keyrepr k.u = k.kv in
   let t: tag k.u = HMAC.hmac k.u.alg kv p in
   if None? (MM.lookup k.log (t,p)) then MM.extend k.log (t,p) ();
   t
 
-val verify: 
+val verify:
   #ip:ipkg -> #i:ip.IK.t {ip.IK.registered i} -> k:key ip i ->
   p:text -> t: tag k.u -> ST bool
   (requires (fun _ -> True))
-  (ensures (fun h0 b h1 -> 
-    modifies Set.empty h0 h1 /\ 
+  (ensures (fun h0 b h1 ->
+    modifies Set.empty h0 h1 /\
     (b /\ ideal /\ ip.IK.honest i ==> k.u.good p)))
 
 // We use the log to correct any verification errors
 let verify #ip #i k p t =
   let verified = HMAC.hmacVerify k.u.alg k.kv p t in
-  if ideal then 
+  if ideal then
     let bad = not(ip.IK.get_honesty i) in
-    match FStar.Monotonic.Map.lookup k.log (t,p) with 
-    | Some _ -> verified        (* genuine MAC *) 
+    match FStar.Monotonic.Map.lookup k.log (t,p) with
+    | Some _ -> verified        (* genuine MAC *)
     | None   -> verified && bad (* forgery, blocked when ideal & honest *)
-  else 
-    verified 
+  else
+    verified
 
 
 /// Now entirely independent of TLS.
-/// 
+///
 /// We'll use something of the form
 ///
 /// let good text =
 ///   exists digest.
 ///     hashed ha digest /\
-///     text = hash ha digest /\ 
+///     text = hash ha digest /\
 ///     witnessed (fun h -> "this is the writer's state is ...")
 ///
 /// - how to deal with agility here?
-/// - which level of abstraction? 
+/// - which level of abstraction?
 
 
 /// TODOs:
 /// - Type0/Type1
 /// - how to pass key-generation-time usage parameters?
 /// - how to guarantee matching goodnesses?
-/// - more specific instantiations? 
+/// - more specific instantiations?
 /// (later) support dynamic key compromise
 
-val coerce_eq2: a: (nat -> Type0) -> b: (nat -> Type0) -> v:a 0{a == b} -> b 0 
-let coerce_eq2 a b v = v // this works; many similar variants did not. 
+val coerce_eq2: a: (nat -> Type0) -> b: (nat -> Type0) -> v:a 0{a == b} -> b 0
+let coerce_eq2 a b v = v // this works; many similar variants did not.
 
 module MR = FStar.Monotonic.RRef
 
 #set-options "--initial_fuel 1 --max_fuel 3 --initial_ifuel 1 --max_ifuel 3"
 open FStar.Tactics
 
-let test 
+let test
   (r:rgn {~(is_tls_rgn r)})
-  (v': bytes) 
+  (v': bytes)
   (t': Hashing.Spec.tag Hashing.SHA256)
-  : 
-  ST unit 
+  :
+  ST unit
   (requires fun h0 -> IK.model)
   (ensures fun h0 _ h1 -> True)
-= 
+=
   let ip = IK.Idx // honest, simple indexes
-    nat 
+    nat
     (fun _ -> True)
     (fun _ -> True)
     (fun _ -> False)
@@ -259,25 +320,25 @@ let test
 
   // testing usability of local packages
   let a = Hashing.SHA256 in
-  let ha_of_i (i:nat) = a in 
-  let good_of_i i v = length v = i in // a property worth MACing! 
+  let ha_of_i (i:nat) = a in
+  let good_of_i i v = length v = i in // a property worth MACing!
   let p = localpkg ip ha_of_i good_of_i in
   // assert (IK.LocalPkg?.info #ip p == info1 ip ha_of_i good_of_i); // provable only with unfolds?
 
   let u = {parent=r; alg=a; good=good_of_i 0} in
-  let u = coerce_eq2 (info1 ip ha_of_i good_of_i) (IK.LocalPkg?.info #ip p) u in 
+  let u = coerce_eq2 (info1 ip ha_of_i good_of_i) (IK.LocalPkg?.info #ip p) u in
   let k0: key ip 0 = (IK.LocalPkg?.create p) 0 u in
 
-  // testing usability of full packages 
+  // testing usability of full packages
   let table = IK.mem_alloc #(i:ip.IK.t{ip.IK.registered i}) (key ip) in
-  let q = pkg ip (fun (_:ip.IK.t) -> a) good_of_i table in 
+  let q = pkg ip (fun (_:ip.IK.t) -> a) good_of_i table in
 
-  let h0 = Mem.get() in 
+  let h0 = Mem.get() in
   // assert(
-  //   let open IK in 
+  //   let open IK in
   //   let log : i_mem_table p.key = itable q.define_table in
   //   let v = MR.m_sel h0 log in
-  //   lemma_mm_forall_init v p.local_invariant h0;  
+  //   lemma_mm_forall_init v p.local_invariant h0;
   //   mm_forall v p.local_invariant h0);
   // assert_norm(q.IK.package_invariant h0);
   //if model then
@@ -285,7 +346,7 @@ let test
 
   assume(q.IK.package_invariant h0);
 
-  //TODO superficial but hard to prove... 
+  //TODO superficial but hard to prove...
   // assume(Monotonic.RRef.m_sel h0 (IK.itable table) == MM.empty_map ip.IK.t (key ip));
   // assert(MM.fresh (IK.itable table) 0 h0);
   // assert(q.IK.define_table == table);
@@ -304,11 +365,11 @@ let test
   let b = verify #ip #0 k v' t' in
   assert(b /\ ideal ==> length v' = 0);
   //assert false; // sanity check
-  ()  
-  
+  ()
+
 (*
 
-/// ------------ older, TLS-specific implementation 
+/// ------------ older, TLS-specific implementation
 
 //17-10-21 ADAPT: should depend only on agility parameter.
 
@@ -327,7 +388,7 @@ let authId id = false // TODO: move to Flags
 type tag (i:id) = tag (alg i)
 
 
- 
+
 // We keep the tag in case we later want to enforce tag authentication
 abstract type entry (i:id) (good: bytes -> Type) =
   | Entry: t:tag i -> p:bytes { authId i ==> good p } -> entry i good
@@ -364,7 +425,7 @@ val coerce: i:id -> good: (bytes -> Type) -> parent: rgn -> kv:keyrepr i -> ST(k
   (ensures (fun h0 k h1 ->
     modifies Set.empty h0 h1 /\
     fresh_subregion (region #i #good k) parent h0 h1 ))
-let coerce i good parent kv = 
+let coerce i good parent kv =
   gen0 i good parent kv
 
 val leak: #i:id -> #good: (bytes -> Type) -> k:key i good {~(authId i)} -> Tot (kv:keyrepr i { kv = keyval k })
@@ -401,4 +462,3 @@ let verify #i #good k p t =
   x &&
   ( not(authId i) || Some? (seq_find (matches p) log))
 *)
-
